Cvc/Defs.lean
@@ -1,0 +1,77 @@
+/-
+Copyright (c) 2023-2025 by the authors listed in the file AUTHORS and their
+institutional affiliations. All rights reserved.
+Released under Apache 2.0 license as described in the file LICENSE.
+Authors: Adrien Champion
+-/
+
+import Cvc.Init
+import Cvc.Srt.Types
+
+
+
+namespace Cvc
+
+
+
+/-- A type-safe cvc term.
+
+This is just a strongly-typed wrapper around an *unsafe term* (`cvc5.Term`). Values of this type can
+only be created in this module. The constructor is therefore private.
+-/
+structure Term (α : Type) extends AsSrt α where
+/-- Private constructor.. -/
+private ofUnsafe' ::
+  /-- Unsafe term accessor. -/
+  toUnsafe : cvc5.Term
+
+
+
+namespace Term
+
+open cvc5 renaming TermManager → Tm
+
+
+
+/-- Cvc term builder transformer monad. -/
+abbrev BuildT (m : Type → Type) :=
+  ExceptT Error (StateT Tm m)
+
+/-- Cvc term builder monad. -/
+abbrev Build := BuildT Id
+
+
+
+/-- Private constructor with implicit `ToSrt α` instance. -/
+private
+def ofUnsafe [AsSrt α] (term : cvc5.Term) : Term α :=
+  Term.ofUnsafe' inferInstance term
+
+/-- Monadic private constructor. -/
+private
+def ofUnsafeM [Monad m] [AsSrt α] (term : m cvc5.Term) : m (Term α) :=
+  Term.ofUnsafe <$> term
+
+
+
+section variable (term : Term α)
+
+instance instToSrt : ToSrt α := term.toToSrt
+
+
+/-- Reframes the type parameter of a term as its `srt : Srt`. -/
+abbrev asSrt : Term term.srt :=
+  term.eq_srt ▸ term
+
+/-- Facilitates pattern-matching on the sort (`Srt`) of a term. -/
+def srtInspect (f : (srt : Srt) → Term srt → γ) : γ :=
+  f term.srt term.asSrt
+
+/-- SMT-LIB string representation. -/
+protected
+def toString (t : Term α) : String :=
+  t.toUnsafe.toString
+
+instance : ToString (Term α) := ⟨Term.toString⟩
+
+end
